

LSP Exam - January 15, 2018

```
> **CVUT FEL (ČVUT) - České vysoké učení technické v Praze | Czech Technical University in Prague**
>
> [ ](2018-01-15_Exam_CN.md) | [English](2018-01-15_Exam_EN.md) | [Čeština](2018-01-15_Exam_CZ.md)
> **AI-Generated Solution** - Reference analysis below
```

Question 4: Signed/Unsigned Bit Value Frequently Tested

Question: What is the decimal value of the 10-bit binary number `10 0000 1111`?

a) **Unsigned:** _____

b) **Two's-complement (signed):** _____

Detailed Solution

...

Binary: 10 0000 1111
Position: 9 8765 4321 0
...

a) Unsigned calculation:

...

$$= 1 \times 2^9 + 0 \times 2^8 + 0 \times 2^7 + 0 \times 2^6 + 0 \times 2^5 + 0 \times 2^4 + 1 \times 2^3 + 1 \times 2^2 + 1 \times 2^1 + 1 \times 2^0$$
$$= 512 + 0 + 0 + 0 + 0 + 0 + 8 + 4 + 2 + 1$$
$$= 527$$

...

b) Two's-complement (signed) calculation:

Method 1 - Direct calculation:

...

MSB weight is negative: $-2^9 + (\text{remaining bits value})$
$$= -512 + (0 \times 2^8 + \dots + 1 \times 2^3 + 1 \times 2^2 + 1 \times 2^1 + 1 \times 2^0)$$
$$= -512 + 15$$
$$= -497$$

...

Method 2 - Invert and add 1:

...

Original: 10 0000 1111
Inverted: 01 1111 0000
Add 1: 01 1111 0001 = 497
So original = -497

...

Question 5: Equivalent Logic Functions Frequently Tested

****Question**:** Mark all logic functions that are equivalent to other functions:

```

```vhdl
f1 <= (A xor C) or (A and not C);
f2 <= (B or C) and (not A or B or C);
f3 <= ((C and not B) or (B and A));
f4 <= (A or C) and (not A or not C);
f5 <= (A and not B) xor (A and C);
f6 <= (A and not C) or (C and not A);
```

```

Solution Method: Karnaugh Map for Each Function

f1 = (A xor C) or (A and not C)

| f1 | C=0 | C=1 |
|-----|-----|-----|
| A=0 | 0 | 1 |
| A=1 | 1 | 1 |

f1 = A + C

f2 = (B or C) and (not A or B or C)

| f2 | BC=00 | BC=01 | BC=11 | BC=10 |
|-----|-------|-------|-------|-------|
| A=0 | 0 | 1 | 1 | 1 |
| A=1 | 0 | 1 | 1 | 0 |

f3 = (C and not B) or (B and A)

| f3 | BC=00 | BC=01 | BC=11 | BC=10 |
|-----|-------|-------|-------|-------|
| A=0 | 0 | 1 | 0 | 0 |
| A=1 | 0 | 1 | 1 | 0 |

f4 = (A or C) and (not A or not C)

| f4 | C=0 | C=1 |
|-----|-----|-----|
| A=0 | 0 | 1 |
| A=1 | 1 | 0 |

****f4 = A C (XOR)****

f5 = (A and not B) xor (A and C)

Requires detailed expansion...

f6 = (A and not C) or (C and not A)

| f6 | C=0 | C=1 |
|-----|-----|-----|
| A=0 | 0 | 1 |

```
| A=1 | 1 | 0 |
```

```
**f6 = A C (XOR)**
```

```
### Conclusion
```

```
**f4 f6** (both equal A XOR C)
```

```
---
```

```
## Question: RS Latch Circuit Simulation Frequently Tested
```

```
**Question**: Given the circuit, write the Q output value for inputs A, B, C at times t0, t1, t2, t3 as
```

```
...
```

```
A = ..0../..1../..1../..1../
```

```
B = ..0../..0../..0../..1../
```

```
C = ..1../..1../..0../..0../
```

```
t0 t1 t2 t3
```

```
...
```

```
### Answer
```

```
...
```

```
Q = ...1.../...0.../...0.../...1.../
```

```
...
```

```
---
```

```
## Question: Shannon Expansion Frequently Tested
```

```
Decompose the function into:
```

```
...
```

```
Q = (not Q and f0(A,B,C)) or (Q and f1(A,B,C))
```

```
...
```

```
### Solution Method
```

```
...
```

```
f0 := f(A,B,C, '0') := (A B) · (B C)
```

```
f1 := f(A,B,C, '1') := (A B)
```

```
...
```

```
### Karnaugh Map for f0
```

```
| f0 | C=0 | C=1 |
```

```
|-----|-----|-----|
```

```
| AB=00 | 0 | 1 |
```

```
| AB=01 | 0 | 0 |
```

```
| AB=11 | 1 | 0 |
```

```
| AB=10 | 0 | 0 |
```

```
### Karnaugh Map for f1
```

```
| f1 | C=0 | C=1 |
```

| AB=00 | 1 | 1 |
|-------|---|---|
| AB=01 | 0 | 0 |
| AB=11 | 1 | 1 |
| AB=10 | 0 | 0 |

Quick Reference

Signed Number Calculation Formula

- n-bit two's complement range: $[-2^{n-1}, 2^{n-1}-1]$
- Negative number calculation: $-2^{n-1} + (\text{remaining bits value})$

Equivalent Function Identification Method

1. Draw Karnaugh map for each function
2. Compare if Karnaugh maps are identical
3. Identical functions are equivalent

Shannon Expansion Formula

$$f(x_1, x_2, \dots, x_n, Q) = \bar{Q} \cdot f_0 + Q \cdot f_1$$

Where:

- $f_0 = f(x_1, x_2, \dots, x_n, 0)$
- $f_1 = f(x_1, x_2, \dots, x_n, 1)$